hachi/benches/genesis/src/lib.rs
@@ -88,3 +88,5 @@ pub mod evalsplit;
 pub mod ringswitch;
 
 pub mod quadeval;
+
+pub mod endpiece;
